MRiscX/Semantics/MsTheory.lean
@@ -19,45 +19,55 @@ can apply these theorems with simp automatically.
 
 namespace MState
 
-@[simp] theorem incPc_increments_pc: ∀ (ms:MState),
+
+
+
+@[simp]
+theorem incPc_increments_pc: ∀ (ms:MState),
   ms.incPc = {ms with pc := ms.pc + 1} := by
   intros ms
   unfold MState.incPc
   simp
 
-@[simp] theorem setReg_incPc_symm: ∀(ms:MState) (r:Registers),
+@[simp]
+theorem setReg_incPc_symm: ∀(ms:MState) (r:Registers),
   (ms.setRegister r).incPc = ms.incPc.setRegister r := by
   intros ms r
   unfold MState.setRegister MState.incPc
   simp
 
-@[simp] theorem addReg_incPc_comm: ∀(ms:MState) (r : RegisterName) (v: UInt64),
+@[simp]
+theorem addReg_incPc_comm: ∀(ms:MState) (r : RegisterName) (v: UInt64),
   (ms.addRegister r v).incPc = ms.incPc.addRegister r v:= by
   intros ms r
   unfold MState.addRegister MState.incPc
   simp
   by_cases h: r.nr = 0 <;> simp [h]
 
-@[simp] theorem addMem_incPc_comm: ∀(ms:MState) (r v: UInt64),
+@[simp]
+theorem addMem_incPc_comm: ∀(ms:MState) (r v: UInt64),
   (ms.addMemory r v).incPc = ms.incPc.addMemory r v:= by
   intros ms r
   unfold MState.addMemory MState.incPc
   simp
 
-@[simp] theorem incPc_terminated: ∀(ms:MState),
+@[simp]
+theorem incPc_terminated: ∀(ms:MState),
   ms.incPc.terminated = ms.terminated := by
   intros ms
   unfold MState.incPc
   simp
 
 
-@[simp] theorem setPc_terminated: ∀(ms:MState) (p:UInt64),
+@[simp]
+theorem setPc_terminated: ∀(ms:MState) (p:UInt64),
   (ms.setPc p).terminated = ms.terminated := by
   intros ms p
   unfold MState.setPc
   simp
 
-@[simp] theorem addReg_terminated: ∀(ms:MState) (r : RegisterName) (v: UInt64),
+@[simp]
+theorem addReg_terminated: ∀(ms:MState) (r : RegisterName) (v: UInt64),
   (ms.addRegister r v).terminated = ms.terminated := by
   intros ms r v
   unfold MState.addRegister
@@ -65,14 +75,15 @@ namespace MState
   by_cases h: r.nr = 0 <;> simp [h]
 
 
-@[simp] theorem addMem_terminated: ∀(ms:MState) (r v: UInt64),
+@[simp]
+theorem addMem_terminated: ∀(ms:MState) (r v: UInt64),
   (ms.addMemory r v).terminated = ms.terminated := by
   intros ms r v
   unfold MState.addMemory
   simp
 
 
--- @[simp] theorem setReg_setMem_symm: ∀(ms:MState) (r:Registers) (m:Memory),
+-- @[simp]  theorem setReg_setMem_symm: ∀(ms:MState) (r:Registers) (m:Memory),
 --  ((ms.setRegister r).setMemory m).incPc = (ms.setRegister r).incPc.setMemory m ∧
 --   (ms.setRegister r).incPc.setMemory m = (ms.incPc.setRegister r).setMemory m ∧
 --   (ms.incPc.setRegister r).setMemory m = (ms.incPc.setMemory m).setRegister r ∧
@@ -82,7 +93,8 @@ namespace MState
 --   unfold MState.setMemory MState.setRegister MState.incPc
 --   simp
 
-@[simp] theorem addRegister_getRegister_neq:
+@[simp]
+theorem addRegister_getRegister_neq:
   ∀(ms:MState) (r1 r2 : RegisterName) (v : UInt64),
   r1 ≠ r2 →
   ((ms.addRegister r1 v).getRegisterAt r2) = (ms.getRegisterAt r2)
@@ -94,7 +106,8 @@ namespace MState
   rw [t_update_neq]; simp at H
   simp [H]
 
-@[simp] theorem addRegister_getRegisterAtNr_neq:
+@[simp]
+theorem addRegister_getRegisterAtNr_neq:
   ∀(ms:MState) (regNr1 regNr2 : RegisterNr) (name  : RegisterName) (v : UInt64),
   name.nr = regNr1 →
   regNr1 ≠ 0 →
@@ -109,7 +122,8 @@ namespace MState
   rw [nrInName]
   simp [neq_z]
 
-@[simp] theorem addRegister_getRegister_eq:
+@[simp]
+theorem addRegister_getRegister_eq:
   ∀(ms:MState) (r1 r2 : RegisterName) (v : UInt64),
   r1.nr ≠ 0 →
   r1 = r2 →
@@ -117,13 +131,11 @@ namespace MState
   := by
   intros ms r1 r2 v neq_z H
   unfold MState.addRegister MState.getRegisterAt
-  -- rw [←H, t_update_eq]
-  by_cases h: r1.nr = 0 <;> simp [h]
-  rw [h] at neq_z
-  contradiction
-  rw [H, t_update_eq]
+  rw [←H]
+  simp [neq_z]
 
-@[simp] theorem addRegister_getRegisterAtNr_eq:
+@[simp]
+theorem addRegister_getRegisterAtNr_eq:
   ∀(ms:MState) (name : RegisterName) (nr : RegisterNr) (v : UInt64),
   nr ≠ 0 →
   name.nr = nr →
@@ -138,7 +150,8 @@ namespace MState
   contradiction
 
 
-@[simp] theorem setPc_getRegister_indep:
+@[simp]
+theorem setPc_getRegister_indep:
   ∀(ms:MState) (i : UInt64) (r : RegisterName),
   ((ms.setPc i).getRegisterAt r) = (ms.getRegisterAt r)
   := by
@@ -146,7 +159,8 @@ namespace MState
   unfold MState.setPc MState.getRegisterAt
   simp
 
-@[simp] theorem setPc_getRegisterAtNr_indep:
+@[simp]
+theorem setPc_getRegisterAtNr_indep:
   ∀(ms:MState) (i : UInt64) (r : RegisterNr),
   ((ms.setPc i).getRegisterAtNr r) = (ms.getRegisterAtNr r)
   := by
@@ -154,7 +168,8 @@ namespace MState
   unfold MState.setPc MState.getRegisterAtNr
   simp
 
-@[simp] theorem setPc_getRegisterAt_def_indep:
+@[simp]
+theorem setPc_getRegisterAt_def_indep:
   ∀(ms:MState) (r : RegisterName) (l: UInt64),
   TMap.get ms.registers r = TMap.get (ms.setPc l).registers r
   := by
@@ -162,7 +177,8 @@ namespace MState
   unfold MState.setPc
   simp
 
-@[simp] theorem setPc_getMemory_indep:
+@[simp]
+theorem setPc_getMemory_indep:
   ∀(ms:MState) (i : UInt64) (r : UInt64),
   ((ms.setPc i).getMemoryAt r) = (ms.getMemoryAt r)
   := by
@@ -170,7 +186,8 @@ namespace MState
   unfold MState.setPc MState.getMemoryAt
   simp
 
-@[simp] theorem setPc_getMemoryAt_def_indep:
+@[simp]
+theorem setPc_getMemoryAt_def_indep:
   ∀(ms:MState) (m l: UInt64),
   TMap.get ms.memory m = TMap.get (ms.setPc l).memory m
   := by
@@ -179,7 +196,8 @@ namespace MState
   simp
 
 
-@[simp] theorem set_pc:
+@[simp]
+theorem set_pc:
   ∀(ms:MState) (i : UInt64) ,
   (ms.setPc i).pc = i
   := by
@@ -187,7 +205,8 @@ namespace MState
   unfold MState.setPc
   simp
 
-@[simp] theorem incPc_getRegister_indep:
+@[simp]
+theorem incPc_getRegister_indep:
   ∀(ms:MState) (r : RegisterName),
   ((ms.incPc).getRegisterAt r) = (ms.getRegisterAt r)
   := by
@@ -195,7 +214,8 @@ namespace MState
   unfold MState.incPc MState.getRegisterAt
   simp
 
-@[simp] theorem incPc_getRegisterAtNr_indep:
+@[simp]
+theorem incPc_getRegisterAtNr_indep:
   ∀(ms:MState) (r : RegisterNr),
   ((ms.incPc).getRegisterAtNr r) = (ms.getRegisterAtNr r)
   := by
@@ -203,20 +223,23 @@ namespace MState
   unfold MState.incPc MState.getRegisterAtNr
   simp
 
-@[simp] theorem jump_set_pc: ∀ (ms:MState) (s:String) (i:UInt64),
+@[simp]
+theorem jump_set_pc: ∀ (ms:MState) (s:String) (i:UInt64),
   (ms.code.labels.get s) = i ->
   (ms.jump s) = {ms with pc := i} := by
   intros ms s i H
   unfold MState.jump
   rw [H]
 
-@[simp] theorem currInstruction_unfold : ∀ (ms:MState),
+@[simp]
+theorem currInstruction_unfold : ∀ (ms:MState),
   ms.currInstruction = ms.code.instructionMap.get (ms.pc) := by
   intros ms
   unfold MState.currInstruction
   simp
 
-@[simp] theorem runNSteps_currInstruction : ∀ (ms:MState) (n:Nat),
+@[simp]
+theorem runNSteps_currInstruction : ∀ (ms:MState) (n:Nat),
   (ms.runNSteps n).currInstruction = (ms.runNSteps n).code.instructionMap.get ((ms.runNSteps n).pc)
   := by
   intros ms n
@@ -226,26 +249,30 @@ namespace MState
 
 
 
-@[simp] theorem addRegister_unfold (ms:MState) : ∀ (r : RegisterName) (v : UInt64),
+@[simp]
+theorem addRegister_unfold (ms:MState) : ∀ (r : RegisterName) (v : UInt64),
   r.nr ≠ 0 →
   ms.addRegister r v = {ms with registers := ((r) ↦ v ; ms.registers)} := by
   intros r val_toUnits_apply H
   unfold MState.addRegister
   simp [H]
 
-@[simp] theorem addMemory_unfold (ms:MState) : ∀ (a v:UInt64),
+@[simp]
+theorem addMemory_unfold (ms:MState) : ∀ (a v:UInt64),
   ms.addMemory a v = {ms with memory :=
     ((a) ↦ v ; ms.memory)} := by
   intros a v
   unfold MState.addMemory
   simp
 
-@[simp] theorem run_zero_steps (ms:MState) :
+@[simp]
+theorem run_zero_steps (ms:MState) :
   ms.runNSteps 0 = ms := by
   unfold MState.runNSteps
   rfl
 
-@[simp] theorem run_n_run_one : ∀ (ms:MState) (n:Nat),
+@[simp]
+theorem run_n_run_one : ∀ (ms:MState) (n:Nat),
   (ms.runNSteps n).runOneStep = ms.runNSteps (n+1) := by
   intros ms n
   revert ms
@@ -260,7 +287,8 @@ namespace MState
     unfold MState.runNSteps
     rw [IHN']
 
-@[simp] theorem run_n_run_one_comm : ∀ (ms:MState) (n:Nat),
+@[simp]
+theorem run_n_run_one_comm : ∀ (ms:MState) (n:Nat),
   (ms.runNSteps n).runOneStep = ms.runOneStep.runNSteps n := by
   intros ms n
   revert ms
@@ -275,13 +303,15 @@ namespace MState
     unfold MState.runNSteps
     rw [IHN']
 
-@[simp] theorem run_one_step_eq_run_n_1 : ∀ (ms:MState),
+@[simp]
+theorem run_one_step_eq_run_n_1 : ∀ (ms:MState),
   ms.runOneStep = ms.runNSteps 1 := by
   intros ms
   unfold MState.runNSteps
   simp
 
-@[simp] theorem run_N_comm : ∀ (ms:MState) (n m:Nat),
+@[simp]
+theorem run_N_comm : ∀ (ms:MState) (n m:Nat),
   (ms.runNSteps n).runNSteps m = (ms.runNSteps m).runNSteps n := by
   intros ms n
   revert ms
@@ -295,7 +325,8 @@ namespace MState
     rw [<- IHN']
     rw [<- MState.run_n_run_one_comm]
 
-@[simp] theorem run_n_m_steps_comp : ∀ (ms:MState) (n m:Nat),
+@[simp]
+theorem run_n_m_steps_comp : ∀ (ms:MState) (n m:Nat),
   (ms.runNSteps n).runNSteps m = ms.runNSteps (n + m) := by
   intros ms n
   revert ms
@@ -309,32 +340,37 @@ namespace MState
     rw [<- MState.run_n_run_one, Nat.add_assoc, <- IHN', Nat.add_comm,
       <- MState.run_n_run_one, <- MState.run_n_run_one_comm]
 
-@[simp] theorem add_reg_code_no_change : ∀ (ms:MState) (r : RegisterName) (v : UInt64),
+@[simp]
+theorem add_reg_code_no_change : ∀ (ms:MState) (r : RegisterName) (v : UInt64),
   (ms.addRegister r v).code = ms.code := by
   intros ms r v
   unfold MState.addRegister
   simp
   by_cases h : r.nr = 0 <;> simp [h]
 
-@[simp] theorem add_mem_code_no_change : ∀ (ms:MState) (r v:UInt64),
+@[simp]
+theorem add_mem_code_no_change : ∀ (ms:MState) (r v:UInt64),
   (ms.addMemory r v).code = ms.code := by
   intros ms r v
   unfold MState.addMemory
   simp
 
-@[simp] theorem set_pc_code_no_change : ∀ (ms:MState) (v:UInt64),
+@[simp]
+theorem set_pc_code_no_change : ∀ (ms:MState) (v:UInt64),
   (ms.setPc v).code = ms.code := by
   intros ms v
   unfold MState.setPc
   simp
 
-@[simp] theorem set_termianted_code_no_change : ∀ (ms:MState) (v:Bool),
+@[simp]
+theorem set_termianted_code_no_change : ∀ (ms:MState) (v:Bool),
   (ms.setTerminated v).code = ms.code := by
   intros ms v
   unfold MState.setTerminated
   simp
 
-@[simp] theorem jump_register_indep: ∀ (ms:MState) (m:Memory) (r:Registers) (c:Code) (s:String),
+@[simp]
+theorem jump_register_indep: ∀ (ms:MState) (m:Memory) (r:Registers) (c:Code) (s:String),
   ({ms with registers := r, memory := m, code := c}.jump s).pc = ({ms with code := c}.jump s).pc := by
   intros ms m r c s
   unfold MState.jump
@@ -343,16 +379,18 @@ namespace MState
   . dsimp
   . simp
 
-@[simp] theorem get_register_only_register: ∀ (m:Memory) (regs:Registers) (c:Code)
-    (terminated:Bool) (regName : RegisterName) (p:UInt64) (ic : Nat),
-  {registers := regs, memory := m, code := c, pc := p,
-    terminated := terminated, instrCounter := ic: MState}.getRegisterAt regName =
-  TMap.get regs regName := by
-  intros r m _ terminated i p
-  unfold MState.getRegisterAt
-  simp
+-- @[simp]
+-- theorem get_register_only_register: ∀ (m:Memory) (regs:Registers) (c:Code)
+--     (terminated:Bool) (regName : RegisterName) (p:UInt64) (ic : Nat),
+--   {registers := regs, memory := m, code := c, pc := p,
+--     terminated := terminated, instrCounter := ic: MState}.getRegisterAt regName =
+--   TMap.get regs regName := by
+--   intros r m _ terminated i p
+--   unfold MState.getRegisterAt
+--   simp
 
-@[simp] theorem get_register_at_nr_only_register: ∀ (m:Memory) (regs:Registers) (c:Code)
+@[simp]
+theorem get_register_at_nr_only_register: ∀ (m:Memory) (regs:Registers) (c:Code)
     (terminated:Bool) (regNr : RegisterNr) (p:UInt64) (ic : Nat),
   {registers := regs, memory := m, code := c, pc := p,
     terminated := terminated, instrCounter := ic : MState}.getRegisterAtNr regNr =
@@ -361,7 +399,8 @@ namespace MState
   unfold MState.getRegisterAtNr
   simp
 
-@[simp] theorem get_register_only_register': ∀ (ms:MState) (m:Memory) (r:Registers) (c:Code)
+@[simp]
+theorem get_register_only_register': ∀ (ms:MState) (m:Memory) (r:Registers) (c:Code)
     (terminated:Bool) (i : RegisterName) (p:UInt64),
   {ms with
     memory := m, registers := r, pc := p, code := c, terminated := terminated }.getRegisterAt i =
@@ -370,7 +409,8 @@ namespace MState
   unfold MState.getRegisterAt
   simp
 
-@[simp] theorem get_register_at_nr_only_register': ∀ (ms:MState) (m:Memory) (r:Registers) (c:Code)
+@[simp]
+theorem get_register_at_nr_only_register': ∀ (ms:MState) (m:Memory) (r:Registers) (c:Code)
     (terminated:Bool) (nr : RegisterNr) (p:UInt64),
   {ms with
     memory := m, registers := r, pc := p, code := c, terminated := terminated }.getRegisterAtNr nr =
@@ -379,7 +419,8 @@ namespace MState
   unfold MState.getRegisterAtNr
   simp
 
-@[simp] theorem get_register_only_memory: ∀ (m:Memory) (r:Registers) (c:Code) (terminated:Bool)
+@[simp]
+theorem get_register_only_memory: ∀ (m:Memory) (r:Registers) (c:Code) (terminated:Bool)
     (i p:UInt64),
   {registers := r, memory := m, code := c, pc := p,
     terminated := terminated, instrCounter := ic : MState}.getMemoryAt i =
@@ -388,7 +429,8 @@ namespace MState
   unfold MState.getMemoryAt
   simp
 
-@[simp] theorem get_register_only_memory': ∀ (ms:MState) (m:Memory) (r:Registers) (c:Code)
+@[simp]
+theorem get_register_only_memory': ∀ (ms:MState) (m:Memory) (r:Registers) (c:Code)
     (terminated:Bool) (i p:UInt64),
   {ms with
     memory := m, registers := r, pc := p, code := c, terminated := terminated }.getMemoryAt i =
@@ -398,18 +440,20 @@ namespace MState
   simp
 
 
-@[simp] theorem get_label_from_code: ∀(ms : MState) (s : String) (l : UInt64),
+@[simp]
+theorem get_label_from_code: ∀(ms : MState) (s : String) (l : UInt64),
   (ms.getLabelAt s = l) = (PMap.get ms.code.labels s = l)
   := by
   intros ms s l
   unfold MState.getLabelAt
   simp
 
-@[simp] theorem getRegisterAt_def: ∀ (ms : MState) (r : RegisterName),
-  ms.getRegisterAt r = TMap.get ms.registers r := by
-  intros ms r
-  unfold MState.getRegisterAt
-  simp
+-- @[simp]
+-- theorem getRegisterAt_def: ∀ (ms : MState) (r : RegisterName),
+--   ms.getRegisterAt r = TMap.get ms.registers r := by
+--   intros ms r
+--   unfold MState.getRegisterAt
+--   simp
 
 -- @[simp] theorem get_register_at_nr_def: ∀ (ms : MState) (r : RegisterNr),
 --   ms.getRegisterAtNr r = TMap.get ms.registers r := by
@@ -417,62 +461,84 @@ namespace MState
 --   unfold MState.getRegisterAt
 --   simp
 
-@[simp] theorem getMemoryAt_def: ∀ (ms : MState) (l : UInt64),
+@[simp]
+theorem getMemoryAt_def: ∀ (ms : MState) (l : UInt64),
   ms.getMemoryAt l = TMap.get ms.memory l := by
   intros ms l
   unfold MState.getMemoryAt
   simp
 
-@[simp] theorem TMap_register_le_zero_eq_zero: ∀(ms:MState) (r : RegisterName),
+@[simp]
+theorem TMap_register_le_zero_eq_zero: ∀(ms:MState) (r : RegisterName),
     (TMap.get ms.registers r ≤ 0) = (TMap.get ms.registers r = 0) := by
   simp
 
-@[simp] theorem register_le_zero_eq_zero: ∀(ms:MState) (r : RegisterName),
+@[simp]
+theorem register_le_zero_eq_zero: ∀(ms:MState) (r : RegisterName),
     (ms.getRegisterAt r ≤ 0) = (ms.getRegisterAt r = 0) := by
   simp
 
-@[simp] theorem register_nr_le_zero_eq_zero: ∀(ms:MState) (r : RegisterNr),
+@[simp]
+theorem register_nr_le_zero_eq_zero: ∀(ms:MState) (r : RegisterNr),
     (ms.getRegisterAtNr r ≤ 0) = (ms.getRegisterAtNr r = 0) := by
   simp
 
-@[simp] theorem incInstrCounter_no_change_in_code: ∀ (ms : MState),
+@[simp]
+theorem reg_zero_not_writeable: ∀ (ms : MState) (name : RegisterName) (v : UInt64),
+  name.nr == 0 →
+  (ms.addRegister name v).getRegisterAt name = ms.getRegisterAt name
+  := by
+  intros ms name v h
+  unfold MState.addRegister
+  rw [h]
+  simp
+
+
+@[simp]
+theorem incInstrCounter_no_change_in_code: ∀ (ms : MState),
   ms.incInstrCounter.code = ms.code
   := by
   unfold MState.incInstrCounter
   simp
 
-@[simp] theorem incInstrCounter_no_change_in_pc: ∀ (ms : MState),
+@[simp]
+theorem incInstrCounter_no_change_in_pc: ∀ (ms : MState),
   ms.incInstrCounter.pc = ms.pc
   := by
   unfold MState.incInstrCounter
   simp
 
-@[simp] theorem incInstrCounter_incPc_comm: ∀ (ms : MState),
+@[simp]
+theorem incInstrCounter_incPc_comm: ∀ (ms : MState),
   ms.incInstrCounter.incPc = ms.incPc.incInstrCounter
   := by
   unfold MState.incInstrCounter
   simp
 
 
-@[simp] theorem incInstrCounter_no_change_mem: ∀ (ms : MState),
+@[simp]
+theorem incInstrCounter_no_change_mem: ∀ (ms : MState),
   ms.incInstrCounter.memory = ms.memory
   := by
   unfold MState.incInstrCounter
   simp
 
-@[simp] theorem incInstrCounter_no_change_registers: ∀ (ms : MState),
+@[simp]
+theorem incInstrCounter_no_change_registers: ∀ (ms : MState),
   ms.incInstrCounter.registers = ms.registers
   := by
   unfold MState.incInstrCounter
   simp
 
-@[simp] theorem incInstrCounter_no_change_terminated: ∀ (ms : MState),
+@[simp]
+theorem incInstrCounter_no_change_terminated: ∀ (ms : MState),
   ms.incInstrCounter.terminated = ms.terminated
   := by
   unfold MState.incInstrCounter
   simp
 
-@[simp] theorem runOneSteps_code_remains : ∀ (ms:MState),
+@[simp]
+theorem runOneSteps_code_remains : ∀ (ms:MState),
   (ms.runOneStep).code = ms.code
   := by
   intros ms
@@ -498,7 +564,8 @@ namespace MState
       all_goals cases PMap.get ms.code.labels lbl <;> simp
 
 
-@[simp] theorem runNSteps_code_remains : ∀ (ms:MState) (n:Nat),
+@[simp]
+theorem runNSteps_code_remains : ∀ (ms:MState) (n:Nat),
   (ms.runNSteps n).code = ms.code
   := by
   intros ms n
@@ -512,7 +579,8 @@ namespace MState
     unfold MState.runNSteps
     exact IHn'
 
-@[simp] theorem code_remains_same : ∀ (ms ms' : MState) (code : Code) (n : ℕ),
+@[simp]
+theorem code_remains_same : ∀ (ms ms' : MState) (code : Code) (n : ℕ),
   ms.code = code →
   ms.runNSteps n = ms' →
   ms'.code = code
